core/V1ModelSpec.v
@@ -3,11 +3,13 @@ Require Import Poulet4.Typed.
 Require Import Poulet4.Syntax.
 Require Import Poulet4.Value.
 Require Import Poulet4.Semantics.
-Require Import ProD3.core.Coqlib.
-Require Import ProD3.core.Hoare.
 Require Import Poulet4.V1Model.
 Require Import Poulet4.P4Notations.
 Require Import Poulet4.P4Arith.
+Require Import ProD3.core.Coqlib.
+Require Import ProD3.core.Hoare.
+Require Import ProD3.core.FuncSpec.
+Require Import ProD3.core.AssertionNotations.
 Require Import BinNat.
 Require Import BinInt.
 Open Scope Z_scope.
@@ -17,29 +19,23 @@ Require Import Hammer.Plugin.Hammer. *)
 Section V1ModelSpec.
 
 Context {tags_t: Type} {tags_t_inhabitant : Inhabitant tags_t}.
-Notation Val := (@ValueBase tags_t bool).
-Notation Sval := (@ValueBase tags_t (option bool)).
+Notation Val := (@ValueBase bool).
+Notation Sval := (@ValueBase (option bool)).
 (* Notation ValSet := (@ValueSet tags_t). *)
 Notation Lval := (@ValueLvalue tags_t).
 
-Notation ident := (P4String.t tags_t).
+Notation ident := string.
 Notation path := (list ident).
-Notation P4Int := (P4Int.t tags_t).
-Notation P4String := (P4String.t tags_t).
-Notation signal := (@signal tags_t).
-Notation Locator := (@Locator tags_t).
 Notation Expression := (@Expression tags_t).
 Notation argument := (@argument tags_t).
 
-Notation extern_state := (@Target.extern_state tags_t Expression V1ModelExternSem).
-
-Notation object := (@object tags_t Expression).
-
 Instance target : @Target tags_t Expression := V1Model.
 
-Variable ge : (@genv tags_t).
+Variable ge : genv.
 
-Definition register_read_pre (p : path) reg i :=
+(* Definition register_read_pre (p : path) reg i :=
+  (0 <= i < reg_size reg)%Z
+  ARG
   fun (args : list Sval) st =>
     (0 <= i < reg_size reg)%Z /\
     args = [ValBaseBit (to_loptbool 32%N i)]
@@ -48,30 +44,22 @@ Definition register_read_pre (p : path) reg i :=
 Definition register_read_post (p : path) reg i :=
   fun (args : list Sval) (retv : Val) st =>
     args = [eval_val_to_sval ge (Znth i (reg_content reg))]
-    /\ PathMap.get p (get_external_state st) = Some (ObjRegister reg).
+    /\ PathMap.get p (get_external_state st) = Some (ObjRegister reg). *)
 
-Definition hoare_func_modifies (ge : genv) (p : path) (func : @fundef tags_t) (vars : list Locator) (exts : list Locator) :=
-  forall st inargs targs st' outargs sig,
-    exec_func ge read_ndetbit p st func targs inargs st' outargs sig ->
-    (forall q, ~(In (LInstance q) vars) -> PathMap.get q (get_memory st) = PathMap.get q (get_memory st'))
-    /\ (forall q, ~(In q (map (loc_to_path p) exts)) -> PathMap.get q (get_memory st) = PathMap.get q (get_memory st')).
+Axiom register_read_spec : forall (p : path) (reg : register) (i : Z) (reg_s : register_static),
+  PathMap.get p (ge_ext ge) = Some (EnvRegister reg_s) ->
+  (0 <= i < snd reg_s)%Z ->
+  hoare_func_spec ge p
+    (ARG [ValBaseBit (to_loptbool 32%N i)]
+    (MEM []
+    (EXT [(p, ObjRegister reg)])))
+    (FExternal "register" "read") nil
+    (ARG_RET [eval_val_to_sval (Znth i reg)] ValBaseNull
+    (MEM []
+    (EXT [])))
+    [] [].
 
-Definition hoare_func_spec (ge : genv) (p : path) (pre : arg_assertion)
-    (func : @fundef tags_t) (targs : list P4Type) (post : arg_ret_assertion)
-    (vars : list Locator) (exts : list Locator) :=
-  hoare_func ge p pre func targs post
-    /\ hoare_func_modifies ge p func vars exts.
-
-Definition register_read_spec : Prop :=
-  forall (p : path) (reg : register) (i : Z),
-    hoare_func_spec ge p
-        (register_read_pre p reg i)
-        (FExternal !"Register" !"read")
-        nil
-        (register_read_post p reg i)
-        [] [].
-
-Definition register_write_pre (p : path) reg i v :=
+(* Definition register_write_pre (p : path) reg i v :=
   fun (args : list Sval) st =>
     (0 <= i < reg_size reg)%Z /\
     args = [ValBaseBit (to_loptbool 32%N i); eval_val_to_sval ge v]
@@ -83,16 +71,23 @@ Definition register_write_post (p : path) reg i v :=
     /\ PathMap.get p (get_external_state st) =
         Some (ObjRegister {| reg_width := reg_width reg;
                              reg_size := reg_size reg;
-                             reg_content := upd_Znth i (reg_content reg) v |}).
+                             reg_content := upd_Znth i (reg_content reg) v |}). *)
 
-Definition register_write_spec : Prop :=
-  forall (p : path) (reg : register) (i : Z) (v : Val),
-    hoare_func_spec ge p
-        (register_write_pre p reg i v)
-        (FExternal !"Register" !"write")
-        nil
-        (register_write_post p reg i v)
-        [] [ LInstance [] ].
+(* We need to say v is a definite value, right? *)
+Axiom register_write_spec : forall (p : path) (reg : register) (i : Z) (v : Val) (reg_s : register_static),
+  PathMap.get p (ge_ext ge) = Some (EnvRegister reg_s) ->
+  (0 <= i < snd reg_s)%Z ->
+  hoare_func_spec ge p
+    (ARG [ValBaseBit (to_loptbool 32%N i); eval_val_to_sval v]
+    (MEM []
+    (EXT [(p, ObjRegister reg)])))
+    (FExternal "register" "write") nil
+    (ARG_RET [] ValBaseNull
+    (MEM []
+    (EXT [(p, ObjRegister (upd_Znth i reg v))])))
+    [] [p].
+
+End V1ModelSpec.
 
 (*
 Several issues:
